Makefile
@@ -133,7 +133,7 @@ CONCUR_FILES= \
   scheduler.v TheSchedule.v sepcomp.v seq_lemmas.v ssromega.v stack.v \
   threads_lemmas.v wf_lemmas.v \
   x86_inj.v x86_safe.v x86_context.v fineConc_x86.v executions.v SC_erasure.v spinlocks.v \
-  sync_preds_defs.v sync_preds.v \
+  sync_preds_defs.v sync_preds.v oracular_refinement.v \
   semax_conc_pred.v xsemax_conc.v semax_conc.v semax_to_juicy_machine.v \
   semax_invariant.v semax_initial.v \
   semax_simlemmas.v cl_step_lemmas.v \
